src/circuit.v
@@ -2,23 +2,22 @@ From research Require Import base.
 From research Require Export action.
 From stdpp Require Import option.
 
-Class Circuit (t m tr : Type) :=
-  { mkCircuit : t
-  ; circuitResult : m -> Type
-  ; circuitCall : forall (method : m), @Action t (circuitResult method)
-  ; circuitTrace : t -> list tr
+Class Circuit (s m tr : Type) :=
+  { mkCircuit : s
+  ; circuitCall : forall (method : m), @Action s unit
+  ; circuitTrace : s -> list tr
   }.
 
-Definition circuitStep `(c : Circuit t m tr) (method : m) (state : t) : t :=
-  default state (runAction2 (circuitCall method) state).
+Definition circuitStep `(c : Circuit s m tr) (method : m) (state : s) : s :=
+  nextState (circuitCall method) state.
 
-Definition circuitSteps `(c : Circuit t m tr) (ms : list m) (state : t) : t :=
+Definition circuitSteps `(c : Circuit s m tr) (ms : list m) (state : s) : s :=
   fold_left (fun st m => circuitStep c m st) ms state.
 
-Definition runCircuit `(c : Circuit t m tr) (ms : list m) : t :=
+Definition runCircuit `(c : Circuit s m tr) (ms : list m) : s :=
   circuitSteps c ms mkCircuit.
 
-Lemma circuitStepsApp `(c: Circuit t m tr) : forall xs1 xs2 st,
+Lemma circuitStepsApp `(c: Circuit s m tr) : forall xs1 xs2 st,
     circuitSteps c (xs1 ++ xs2) st =
       circuitSteps c xs2 (circuitSteps c xs1 st).
 Proof.
@@ -28,7 +27,7 @@ Proof.
   equality.
 Qed.
 
-Lemma runCircuitApp `(c: Circuit t m tr) : forall xs1 xs2,
+Lemma runCircuitApp `(c: Circuit s m tr) : forall xs1 xs2,
     runCircuit c (xs1 ++ xs2) =
       circuitSteps c xs2 (runCircuit c xs1).
 Proof.
@@ -37,36 +36,40 @@ Proof.
   apply circuitStepsApp.
 Qed.
 
-Definition simulates
-  `(c1: Circuit t1 m1 tr)
-  `(c2: Circuit t2 m2 tr)
-  policy
-  (R : t1 -> t2 -> Prop) :=
-  forall s1 s2,
-    R s1 s2 ->
-    (forall m s1' s2',
-        s1' = circuitStep c1 m s1 ->
-        s2' = circuitStep c2 (policy m) s2 ->
-        R s1' s2').
+Definition simulates {s1 s2 t1 t2} a1 a2 (R : s1 -> s2 -> Prop) :=
+  forall st1 st2,
+    R st1 st2 ->
+    (forall st1' st2',
+        st1' = nextState (a := t1) a1 st1 ->
+        st2' = nextState (a := t2) a2 st2 ->
+        R st1' st2').
 
-Notation "c1 ∼ c2 : policy ; R" := (simulates c1 c2 policy R) (at level 60, c2 at next level).
+Notation "m1 ≺ m2 : R" := (simulates m1 m2 R) (at level 60, m2 at next level).
+
+Definition circuitSimulates `(c1: Circuit s1 m1 tr) `(c2: Circuit s2 m2 tr) p R
+  := forall m, c1.(circuitCall) m ≺ c2.(circuitCall) (p m) : R.
+
+Notation "c1 ∼ c2 : policy ; R" :=
+  (circuitSimulates c1 c2 policy R) (at level 60, c2 at next level).
 
 (* We say a circuit [c] is constant time relevant to some policy [policy],
    if given the set of method calls to [c], we get the specification leakage
    by applying policy [policy] to the series of method calls. If from the specification
    leakage we can determine the implementation leakage trace, we get constant time
    wrt [policy]. *)
-Definition constantTime {m2} `(c : Circuit t m1 tr) (policy : list m1 -> list m2) :=
+Definition constantTime {m2} `(c : Circuit s m1 tr) (policy : list m1 -> list m2) :=
   exists f, forall xs, circuitTrace (runCircuit c xs) = f (policy xs).
 
-Lemma simulationConstantTime `(c1 : Circuit t1 m1 tr) `(c2 : Circuit t2 m2 tr) policy :
+Lemma circuitConstantTime
+  `(c1 : Circuit s1 m1 tr)
+  `(c2 : Circuit s2 m2 tr) policy :
   forall R, (c1 ∼ c2 : policy; R) ->
        R c1.(mkCircuit) c2.(mkCircuit) ->
-       (forall t1 t2, R t1 t2 -> c1.(circuitTrace) t1 = c2.(circuitTrace) t2) ->
+       (forall st1 st2, R st1 st2 -> c1.(circuitTrace) st1 = c2.(circuitTrace) st2) ->
        constantTime c1 (map policy).
 Proof.
   intros R Hsimulates Hinit Htrace.
-  cbv [ constantTime simulates ] in *.
+  cbv [ constantTime circuitSimulates simulates ] in *.
   exists (fun zs => circuitTrace (runCircuit c2 zs)).
   intros.
   apply Htrace.
@@ -75,10 +78,9 @@ Proof.
   - rewrite map_app.
     rewrite !runCircuitApp.
     simplify.
-    apply Hsimulates with
-      (s1 := runCircuit c1 xs)
-      (s2 := runCircuit c2 (map policy xs))
-      (m := x); equality.
+    set (st1 := runCircuit c1 xs) in *.
+    set (st2 := runCircuit c2 (map policy xs)) in *.
+    apply Hsimulates with (st1 := st1) (st2 := st2) (m := x); equality.
 Qed.
 
 Arguments Circuit {_ _ _}.
