src/multiplier.v
@@ -1,229 +1,250 @@
 From research Require Import base bit circuit.
 
-Notation Maybe := @option.
+Section WithContext.
+  Inductive specLeakage :=
+  | Spec__Enq (a : Bit 8)
+  | Spec__Deq
+  | Spec__Rule.
 
-Inductive specLeakage :=
-| SpecLeakage__Enq (a : Bit 4)
-| SpecLeakage__Deq
-| SpecLeakage__Rule.
+  Inductive implLeakage :=
+  | Impl__Enq
+  | Impl__Deq
+  | Impl__Rule.
 
-Inductive implLeakage :=
-| ImplLeakage__Enq
-| ImplLeakage__Deq
-| ImplLeakage__Rule.
+  Inductive method :=
+  | Enq (a b : Bit 8)
+  | Deq
+  | Rule.
 
-Inductive method :=
-| Enq (a b : Bit 4)
-| Deq
-| Rule.
+  Inductive state :=
+  | State__Empty
+  | State__Busy
+  | State__Full.
 
-Inductive state :=
-| State__Empty
-| State__Busy
-| State__Full.
+  Instance state__EqDecision : EqDecision state. solve_decision. Defined.
 
-Instance state__EqDecision : EqDecision state. solve_decision. Defined.
+  Record Multiplier :=
+    { multiplierA     : Bit 8
+    ; multiplierB     : Bit 8
+    ; multiplierC     : Bit 3
+    ; multiplierP     : Bit 16
+    ; multiplierSt    : state
+    ; multiplierTrace : list implLeakage
+    }.
 
-Record Multiplier :=
-  { multiplierA : Bit 4
-  ; multiplierB : Bit 4
-  ; multiplierC : Bit 2
-  ; multiplierP : Bit 8
-  ; multiplierSt : state
-  ; multiplierTrace : list implLeakage
-  }.
+  Definition mkMultiplier :=
+    {|
+      multiplierA     := 0%bv;
+      multiplierB     := 0%bv;
+      multiplierC     := 0%bv;
+      multiplierP     := 0%bv;
+      multiplierSt    := State__Empty;
+      multiplierTrace := []
+    |}.
 
-Definition mkMultiplier :=
-  {|
-    multiplierA := 0%bv;
-    multiplierB := 0%bv;
-    multiplierC := 0%bv;
-    multiplierP := 0%bv;
-    multiplierSt := State__Empty;
-    multiplierTrace := []
-  |}.
+  Definition multiplierEmpty st :=
+    bool_decide (st.(multiplierSt) = State__Empty).
 
-Definition multiplierEmpty st := bool_decide (st.(multiplierSt) = State__Empty).
-Definition multiplierBusy st := bool_decide (st.(multiplierSt) = State__Busy).
-Definition multiplierFull st := bool_decide (st.(multiplierSt) = State__Full).
+  Definition multiplierBusy st :=
+    bool_decide (st.(multiplierSt) = State__Busy).
 
-Definition multiplierEnq x1 x2 : Action unit :=
-  guard
-    {{ multiplierEmpty }}
-    {{ let%modify _ := snoc ImplLeakage__Enq on multiplierTrace in
-       let%write  _ := x1 on multiplierA in
-       let%write  _ := x2 on multiplierB in
-       let%write  _ := 0%bv on multiplierC in
-       let%write  _ := 0%bv on multiplierP in
-       let%write  _ := State__Busy on multiplierSt in
-       pass
-    }}.
+  Definition multiplierFull st :=
+    bool_decide (st.(multiplierSt) = State__Full).
 
-Definition multiplierDeq : Action (Bit 8) :=
-  guard
-    {{ multiplierFull }}
-    {{ let%read p  := multiplierP  in
-       let%modify _ := snoc ImplLeakage__Deq on multiplierTrace in
-       let%write _ := State__Empty on multiplierSt in
-       ret p
-    }}.
+  Definition multiplierEnq x1 x2 :=
+    guard
+      {{ multiplierEmpty }}
+      {{ let%modify _ := cons Impl__Enq on multiplierTrace in
+         let%write  _ := x1 on multiplierA in
+         let%write  _ := x2 on multiplierB in
+         let%write  _ := 0%bv on multiplierC in
+         let%write  _ := 0%bv on multiplierP in
+         let%write  _ := State__Busy on multiplierSt in
+         pass
+      }}.
 
-Definition multiplierShiftAndAdd : Action unit :=
-  {{ let%read a := multiplierA in
-     let%read b := multiplierB in
-     let%read c := multiplierC in
-     let%read p := multiplierP in
-     when decide (a <> 0%bv) then
-       let t :=
-         if decide (truncate1 a = 1)%bv then
-           zeroExtend (z := 8) b
-         else
-           0%bv
-       in
-       let%write _ := (p + (t ≪ zeroExtend c))%bv on multiplierP in
-       let%write _ := (a ≫ 1)%bv on multiplierA in
-       let%write _ := (c + 1)%bv on multiplierC in
-       pass
-  }}.
+  Definition multiplierFirst st := st.(multiplierP).
 
-Definition multiplierRule : Action unit :=
-  guard
-    {{ multiplierBusy }}
+  Definition multiplierDeq :=
+    guard
+      {{ multiplierFull }}
+      {{ let%read p := multiplierP  in
+         let%modify _ := cons Impl__Deq on multiplierTrace in
+         let%write _ := State__Empty on multiplierSt in
+         pass
+      }}.
+
+  Definition multiplierShiftAndAdd : Action unit :=
     {{ let%read a := multiplierA in
-       let%modify _ := snoc ImplLeakage__Rule on multiplierTrace in
-       if decide (a = 0%bv) then
-         let%write _ := State__Full on multiplierSt in
+       let%read b := multiplierB in
+       let%read c := multiplierC in
+       let%read p := multiplierP in
+       when decide (a <> 0%bv) then
+         let t :=
+           if decide (truncate1 a = 1)%bv then
+             zeroExtend b
+           else
+             (16`0x00)%bv
+         in
+         let%write _ := (p + (t ≪ zeroExtend c))%bv on multiplierP in
+         let%write _ := (a ≫ 1)%bv on multiplierA in
+         let%write _ := (c + 1)%bv on multiplierC in
          pass
-       else
-         multiplierShiftAndAdd
     }}.
 
-Instance multiplierCircuit : Circuit :=
-  {|
-    mkCircuit := mkMultiplier;
-    circuitResult m :=
-      match m with
-      | Enq _ _ => unit
-      | Deq => Bit 8
-      | Rule => unit
-      end;
-    circuitCall m :=
-      match m with
-      | Enq a b => multiplierEnq a b
-      | Deq => multiplierDeq
-      | Rule => multiplierRule
-      end;
-    circuitTrace := multiplierTrace
-  |}.
+  Definition multiplierRule : Action unit :=
+    guard
+      {{ multiplierBusy }}
+      {{ let%read a := multiplierA in
+         let%modify _ := cons Impl__Rule on multiplierTrace in
+         if decide (a = 0%bv) then
+           let%write _ := State__Full on multiplierSt in
+           pass
+         else
+           multiplierShiftAndAdd
+      }}.
 
-Record MultiplierSpec :=
-  { multiplierSpecSt : state
-  ; multiplierSpecA : Bit 4
-  ; multiplierSpecTrace : list implLeakage
-  }.
+  Instance multiplierCircuit : Circuit :=
+    {|
+      mkCircuit := mkMultiplier;
+      circuitCall m :=
+        match m with
+        | Enq a b => multiplierEnq a b
+        | Deq => multiplierDeq
+        | Rule => multiplierRule
+        end;
+      circuitTrace := multiplierTrace
+    |}.
 
-Definition mkMultiplierSpec :=
-  {|
-    multiplierSpecSt := State__Empty;
-    multiplierSpecA := 0%bv;
-    multiplierSpecTrace := []
-  |}.
+  Record MultiplierSpec :=
+    { multiplierSpecSt    : state
+    ; multiplierSpecA     : Bit 8
+    ; multiplierSpecTrace : list implLeakage
+    }.
 
-Definition multiplierSpecEmpty st := bool_decide (st.(multiplierSpecSt) = State__Empty).
-Definition multiplierSpecBusy st := bool_decide (st.(multiplierSpecSt) = State__Busy).
-Definition multiplierSpecFull st := bool_decide (st.(multiplierSpecSt) = State__Full).
+  Definition mkMultiplierSpec :=
+    {|
+      multiplierSpecSt    := State__Empty;
+      multiplierSpecA     := 0%bv;
+      multiplierSpecTrace := []
+    |}.
 
-Definition multiplierSpecEnq in__a :=
-  guard
-    {{ multiplierSpecEmpty }}
-    {{ let%modify _ := snoc ImplLeakage__Enq on multiplierSpecTrace in
-       let%write _ := in__a on multiplierSpecA in
-       let%write _ := State__Busy on multiplierSpecSt in
-       pass
-    }}.
+  Definition multiplierSpecEmpty st :=
+    bool_decide (st.(multiplierSpecSt) = State__Empty).
 
-Definition multiplierSpecDeq :=
-  guard
-    {{ multiplierSpecFull }}
-    {{ let%modify _ := snoc ImplLeakage__Deq on multiplierSpecTrace in
-       let%write _ := State__Empty on multiplierSpecSt in
-       pass
-    }}.
+  Definition multiplierSpecBusy st :=
+    bool_decide (st.(multiplierSpecSt) = State__Busy).
 
-Definition multiplierSpecShift :=
-  {{ let%read a := multiplierSpecA in
-     when decide (a <> 0%bv) then
-       let%write _ := (a ≫ 1)%bv on multiplierSpecA in
-       pass
-  }}.
+  Definition multiplierSpecFull st :=
+    bool_decide (st.(multiplierSpecSt) = State__Full).
 
-Definition multiplierSpecRule :=
-  guard
-    {{ multiplierSpecBusy }}
+  Definition multiplierSpecEnq in__a :=
+    guard
+      {{ multiplierSpecEmpty }}
+      {{ let%modify _ := cons Impl__Enq on multiplierSpecTrace in
+         let%write _ := in__a on multiplierSpecA in
+         let%write _ := State__Busy on multiplierSpecSt in
+         pass
+      }}.
+
+  Definition multiplierSpecDeq :=
+    guard
+      {{ multiplierSpecFull }}
+      {{ let%modify _ := cons Impl__Deq on multiplierSpecTrace in
+         let%write _ := State__Empty on multiplierSpecSt in
+         pass
+      }}.
+
+  Definition multiplierSpecShift :=
     {{ let%read a := multiplierSpecA in
-       let%modify _ := snoc ImplLeakage__Rule on multiplierSpecTrace in
-       if decide (a = 0%bv) then
-         let%write _ := State__Full on multiplierSpecSt in
+       when decide (a <> 0%bv) then
+         let%write _ := (a ≫ 1)%bv on multiplierSpecA in
          pass
-       else
-         multiplierSpecShift
     }}.
 
-Instance multiplierSpecCircuit : Circuit :=
-  {|
-    mkCircuit := mkMultiplierSpec;
-    circuitResult m := unit;
-    circuitCall m :=
-      match m with
-      | SpecLeakage__Enq a => multiplierSpecEnq a
-      | SpecLeakage__Deq => multiplierSpecDeq
-      | SpecLeakage__Rule => multiplierSpecRule
-      end;
-    circuitTrace := multiplierSpecTrace
-  |}.
+  Definition multiplierSpecRule :=
+    guard
+      {{ multiplierSpecBusy }}
+      {{ let%read a := multiplierSpecA in
+         let%modify _ := cons Impl__Rule on multiplierSpecTrace in
+         if decide (a = 0%bv) then
+           let%write _ := State__Full on multiplierSpecSt in
+           pass
+         else
+           multiplierSpecShift
+      }}.
 
-Definition policy1 m :=
-  match m with
-  | Enq a b => SpecLeakage__Enq a
-  | Deq => SpecLeakage__Deq
-  | Rule => SpecLeakage__Rule
-  end.
+  Instance multiplierSpecCircuit : Circuit :=
+    {|
+      mkCircuit := mkMultiplierSpec;
+      circuitCall m :=
+        match m with
+        | Spec__Enq a => multiplierSpecEnq a
+        | Spec__Deq => multiplierSpecDeq
+        | Spec__Rule => multiplierSpecRule
+        end;
+      circuitTrace := multiplierSpecTrace
+    |}.
 
-Definition policy := map policy1.
+  Definition policy1 m :=
+    match m with
+    | Enq a b => Spec__Enq a
+    | Deq => Spec__Deq
+    | Rule => Spec__Rule
+    end.
 
-Definition inv (s1 : Multiplier) (s2 : MultiplierSpec) :=
-  s1.(multiplierSt) = s2.(multiplierSpecSt) /\
-    s1.(multiplierA) = s2.(multiplierSpecA) /\
-    s1.(multiplierTrace) = s2.(multiplierSpecTrace).
+  Definition policy := map policy1.
 
-Local Ltac t0 :=
-  match goal with
-  | m : method |- _ => destruct m
-  | |- context [ decide _ ] => case_decide
-  | |- context [ bool_decide _ ] => case_bool_decide
-  | _ => progress simplify
-  end.
+  Definition rel (s1 : Multiplier) (s2 : MultiplierSpec) :=
+    s1.(multiplierSt) = s2.(multiplierSpecSt) /\
+      s1.(multiplierA) = s2.(multiplierSpecA) /\
+      s1.(multiplierTrace) = s2.(multiplierSpecTrace).
 
-Local Hint Unfold
-  multiplierEnq multiplierSpecEnq
-  multiplierDeq multiplierSpecDeq
-  multiplierRule multiplierSpecRule
-  multiplierShiftAndAdd multiplierSpecShift
-  multiplierEmpty multiplierSpecEmpty
-  multiplierBusy multiplierSpecBusy
-  multiplierFull multiplierSpecFull
-  circuitStep inv : core.
+  Local Hint Unfold
+    multiplierShiftAndAdd multiplierSpecShift
+    multiplierEmpty multiplierSpecEmpty
+    multiplierBusy multiplierSpecBusy
+    multiplierFull multiplierSpecFull : core.
 
-Local Ltac t := repeat t0; solve [ equality | eauto 8 ].
+  Local Hint Unfold rel circuitStep : core.
 
-Theorem simulatesOk : multiplierCircuit ∼ multiplierSpecCircuit : policy1; inv.
-Proof.
-  cbv [ simulates ]; t.
-Qed.
+  Local Ltac t0 :=
+    match goal with
+    | m : method |- _ => destruct m
+    | |- context [ decide _ ] => case_decide
+    | |- context [ bool_decide _ ] => case_bool_decide
+    | |- _ ≺ _ : _ => try eauto 8
+    | _ => progress simplify
+    end.
 
-Local Hint Resolve simulatesOk : core.
+  Local Ltac t := repeat t0; solve [ equality | eauto 8 ].
 
-Theorem constantTimeOk : constantTime multiplierCircuit policy.
-Proof.
-  apply simulationConstantTime with (R := inv) (c2 := multiplierSpecCircuit); t.
-Qed.
+  Lemma multiplierEnqOk : forall a b, multiplierEnq a b ≺ multiplierSpecEnq a : rel.
+  Proof.
+    cbv [ simulates multiplierEnq multiplierSpecEnq ]; t.
+  Qed.
+
+  Lemma multiplierDeqOk : multiplierDeq ≺ multiplierSpecDeq : rel.
+  Proof.
+    cbv [ simulates multiplierDeq multiplierSpecDeq ]; t.
+  Qed.
+
+  Lemma multiplierRuleOk : multiplierRule ≺ multiplierSpecRule : rel.
+  Proof.
+    cbv [ simulates multiplierRule multiplierSpecRule ]; t.
+  Qed.
+
+  Local Hint Resolve multiplierEnqOk multiplierDeqOk multiplierRuleOk : core.
+
+  Theorem multiplierSimulatesOk : multiplierCircuit ∼ multiplierSpecCircuit : policy1; rel.
+  Proof.
+    cbv [ circuitSimulates ]; t.
+  Qed.
+
+  Local Hint Resolve multiplierSimulatesOk : core.
+
+  Theorem multiplierConstantTime : constantTime multiplierCircuit policy.
+  Proof.
+    apply circuitConstantTime with (R := rel) (c2 := multiplierSpecCircuit); t.
+  Qed.
+End WithContext.
