src/regfile.v
@@ -4,12 +4,15 @@ From stdpp Require Import fin finite vector.
 Section WithContext.
   Context (b : N) (sz : N).
 
-  Record RegFile := { regFileContents : Vector (Bit b) (card (Bit sz)) }.
+  Record RegFile := { regFileContents : vec (Bit b) (card (Bit sz)) }.
 
-  Definition mkRegFile := {| regFileContents := mkVector δ (card (Bit sz)) |}.
+  Definition mkRegFile := {| regFileContents := fun_to_vec (const δ) |}.
 
   Definition regFileSub (addr : Bit sz) (t : RegFile) :=
-    if decide (addr = δ)%bv then δ else t.(regFileContents) !!! encode_fin addr.
+    if decide (addr = δ)%bv then
+      δ
+    else
+      t.(regFileContents) !!! encode_fin addr.
 
   Definition regFileUpd (addr : Bit sz) (data : Bit b) :=
     {{ let%modify _ := vinsert (encode_fin addr) data on regFileContents in
